Given the transformation $\mathbf{T}^{-1}\mathbf{AT}=\mathbf{\Lambda}$:
\begin{eqnarray*}
	\mathbf{A}t & = & (\mathbf{T\Lambda T}^{-1}) \\
	\mathbf{A}^nt^n & = & (\mathbf{T\Lambda T}^{-1})(\mathbf{T\Lambda T}^{-1})\ldots(\mathbf{T\Lambda T}^{-1})t^n \\
	                & = & \mathbf{T\Lambda T}^{-1}\mathbf{T\Lambda T}^{-1}\ldots\mathbf{T\Lambda T}^{-1}t^n \\
	\mathbf{A}^nt^n & = & \mathbf{T\Lambda}\mathbf{I}\mathbf{\Lambda I}\ldots\mathbf{I\Lambda T}^{-1}t^n \\
	\               & = & \mathbf{T\Lambda}^n\mathbf{T}^{-1}t^n \\
\end{eqnarray*}
\endinput

%%% Local Variables: 
%%% mode: latex
%%% TeX-master: "notes"
%%% End: