Since,
\[
u = r - \mathbf{Kx}
\]
then the closed-loop system is:
\begin{eqnarray*}
	\dot{\mathbf{x}} & = & \mathbf{A}\mathbf{x}+\mathbf{B}u;\ y = \mathbf{C}\mathbf{x}+\mathbf{D}u \\
	\dot{\mathbf{x}} & = & \mathbf{A}\mathbf{x}+\mathbf{B}(r - \mathbf{K}\mathbf{x});\ y = \mathbf{C}\mathbf{x}+\mathbf{D}(r - \mathbf{K}\mathbf{x}) \\
	\dot{\mathbf{x}} & = & (\mathbf{A}-\mathbf{B}\mathbf{K})\mathbf{x}+\mathbf{B}r;\ y = (\mathbf{C}-\mathbf{D}\mathbf{K})\mathbf{x}+\mathbf{D}r \\
\end{eqnarray*}

\endinput

%%% Local Variables: 
%%% mode: latex
%%% TeX-master: "notes"
%%% End: