Suppose the desired CE is:
\begin{eqnarray}
	\alpha_c(s) & = & (s-p_1)(s-p_2)\cdots(s-p_n)=0 \nonumber \\
	\alpha_c(s) & = & s^n + \alpha_1s^{n-1} + \alpha_2s^{n-2} + \cdots + \alpha_n = 0 \label{eq:6}
\end{eqnarray}

Matching coefficients in Eqs. (\ref{eq:5})  and (\ref{eq:6})  is now simple:
\begin{eqnarray*}
	s^{n - 1}  & : & a_1  + k_1  = \alpha _1  \to k_1  = \alpha _1  - a_1 \\
	s^{n - 2}  & : & a_2  + k_2  = \alpha _2  \to k_2  = \alpha _2  - a_2 \\
	\mathrm{etc}  \\
	s^{0}  & : & a_n  + k_n  = \alpha _n  \to k_n  = \alpha _n  - a_n				
\end{eqnarray*}

\endinput

%%% Local Variables: 
%%% mode: latex
%%% TeX-master: "notes"
%%% End: