In this configuration the observer is driven by:
\[
\tilde E =  Y + R
\] 
Hence the observer dynamics are:
\[
s\hat{\mathbf{X}}=\mathbf{A}\hat{\mathbf{X}}+\mathbf{B}U+\mathbf{L}(\tilde E - \mathbf{C}\hat{\mathbf{X}})
\]
therefore,
\begin{eqnarray*}
	\underbrace {\left( {s{\bf{I}} - {\bf{A}} + {\bf{LC}}} \right)}_{\bf{M}}{\bf{\hat X}} & = & {\bf{B}}U + {\bf{L}}\tilde E \\
	{\bf{\hat X}} & = & {\bf{M}}^{ - 1} {\bf{B}}U + {\bf{M}}^{ - 1} {\bf{L}}\tilde E
\end{eqnarray*}



\endinput

%%% Local Variables: 
%%% mode: latex
%%% TeX-master: "notes"
%%% End: