Taking Laplace transforms, ignoring ICs:
\begin{eqnarray*}
s\hat{\mathbf{X}}(s) & = & (\mathbf{A} - \mathbf{LC} - \mathbf{BK})\hat{\mathbf{X}}(s) + \mathbf{L}Y(s) \\	
\underbrace {(s{\bf{I}} - {\bf{A}} + {\bf{BK}} + {\bf{LC}})}_{{\bf{M + BK}}}{\bf{\hat X}}(s) & = & {\bf{L}}Y(s) \\
\hat{\mathbf{X}}(s) & = & (\mathbf{M}+\mathbf{BK})^{-1}{\bf{L}}Y(s)
\end{eqnarray*}
where $\mathbf{M}=s\mathbf{I}-\mathbf{A}+\mathbf{LC}$.
 
\[
U(s)=-\mathbf{K}\hat{\mathbf{X}}(s)=-\mathbf{K}(\mathbf{M}+\mathbf{BK})^{-1}\mathbf{L}Y(s)
\]
therefore the compensator TF is:
\[
H(s)=-\frac{U(s)}{Y(s)}=\mathbf{K}(\mathbf{M}+\mathbf{BK})^{-1}\mathbf{L}
\]



\endinput

%%% Local Variables: 
%%% mode: latex
%%% TeX-master: "notes"
%%% End: