Let the error in the estimated states $\hat{\mathbf{x}}$ be:
\[
\mathbf{e}=\mathbf{x}-\hat{\mathbf{x}}
\]
then
\[
\frac{d\mathbf{e}}{dt}=\frac{d\mathbf{x}}{dt}-\frac{d\hat{\mathbf{x}}}{dt}
\]

Given,
\[
\frac{d\mathbf{x}}{dt}=\mathbf{A}\mathbf{x}+\mathbf{B}u\ \mathrm{and}\ y=\mathbf{C}\mathbf{x}
\] 
then
\begin{eqnarray*}
	\frac{d\mathbf{e}}{dt} & = & \left(\mathbf{A}\mathbf{x}+\mathbf{B}u\right)-\left\{\mathbf{A}\hat{\mathbf{x}}+\mathbf{B}u+\mathbf{L}(y-\mathbf{C}\hat{\mathbf{x}})\right\} \\
	& = & \mathbf{A}(\mathbf{x}-\hat{\mathbf{x}})-\mathbf{L}(\mathbf{C}\mathbf{x}-\mathbf{C}\hat{\mathbf{x}}) = \mathbf{Ae}-\mathbf{LCe}\\
	& = & (\mathbf{A}-\mathbf{LC})\mathbf{e}
\end{eqnarray*}


\endinput

%%% Local Variables: 
%%% mode: latex
%%% TeX-master: "notes"
%%% End: