The poles of the observer are the roots of the CE:
\[
s^n+(a_1+l_1)s^{n-1}+\cdots+(a_n=l_n)=0
\]
 

If the desired observer poles are at  $s=p_1,p_2,\ldots,p_n$ 
then the desired CE equation is:
\begin{eqnarray*}
	\alpha_e(s) & = & (s-p_1)(s-p_2)\cdots(s-p_n) \\
	            & = & s^n + \alpha_1s^{n-1} + \cdots + \alpha_n = 0
\end{eqnarray*}
 

The  l  coefficients may be found by matching the two equations above. 
Thus,
\[
l_1=\alpha_1-a_1,\ l_2=\alpha_2-a_2,\ \cdots\ l_n=\alpha_n-a_n.
\]


 
 

\endinput

%%% Local Variables: 
%%% mode: latex
%%% TeX-master: "notes"
%%% End: